@@ -1,23 +1,23 @@
 import Flow.Lang.Defs
 
 inductive NodeKind where
-| entry
-| exit
-| skip
-| assign (x : String) (e : Expr)
-| varDecl (x : String)
-| cond (c : Expr)
+| Assign (x : String) (e : Expr)
+| Decl (x : String) (e : Expr)
+| Cond (c : Expr)
+| Skip
 deriving DecidableEq, Repr
 
+abbrev NodeID := Nat
+
 inductive EdgeKind where
-| normal
-| trueBranch
-| falseBranch
+| Normal
+| TBranch
+| FBranch
 deriving DecidableEq, Repr
 
 structure Edge where
-  src : Nat
-  dst : Nat
+  src : NodeID
+  dst : NodeID
   kind : EdgeKind
 deriving DecidableEq, Repr
 
@@ -25,143 +25,72 @@ structure CFG where
   nodes : List NodeKind
   edges : List Edge
   entry : Nat
-  exit  : Nat
-
-def CFG.nodeKind (g : CFG) (n : Nat) : Option NodeKind :=
-  g.nodes[n]?
-
-def CFG.succ (g : CFG) (n : Nat) : List Nat :=
-  g.edges.filterMap (fun ⟨src, dst, _⟩ => if dst = n then some src else none)
-
-def CFG.pred (g : CFG) (n : Nat) : List Nat :=
-  g.edges.filterMap (fun ⟨src, dst, _⟩ => if src = n then some dst else none)
-
-structure CFGBuilder where
-  cfg : CFG
-  nextId : Nat
-
-namespace CFGBuilder
-
-def empty : CFGBuilder where
-  cfg := ⟨[], [], 0, 0⟩
-  nextId := 0
-
-def addNode (b : CFGBuilder) (label : NodeKind) : CFGBuilder × Nat :=
-  let id := b.nextId
-  let b' := { b with
-    cfg := { b.cfg with nodes := b.cfg.nodes ++ [label] }
-    nextId := b.nextId + 1 }
-  (b', id)
-
-/-- Add an edge. -/
-def addEdge (b : CFGBuilder) (src dst : Nat) (label : EdgeKind := .normal) :
-    CFGBuilder :=
-  { b with cfg := { b.cfg with edges := b.cfg.edges ++ [⟨src, dst, label⟩] } }
-
-end CFGBuilder
-
-structure BuildResult where
-  builder : CFGBuilder
-  entry : Nat
   exit : Nat
 
-namespace BuildResult
+namespace CFG
+def nodeKind (g : CFG) (n : NodeID) : Option NodeKind :=
+  g.nodes[n]?
+def succ (g : CFG) (n : NodeID) : List NodeID :=
+  g.edges.filterMap (fun ⟨src, dst, _⟩ => if src = n then dst else none)
+def pred (g : CFG) (n : NodeID) : List NodeID :=
+  g.edges.filterMap (fun ⟨src, dst, _⟩ => if dst = n then src else none)
+def hasEdge (g : CFG) (src dst : NodeID) (k : EdgeKind) : Prop :=
+  ⟨src, dst, k⟩ ∈ g.edges
+end CFG
 
-def single (k : NodeKind) : BuildResult :=
-  let (b, enid) := CFGBuilder.empty.addNode .entry
-  let (b, stid) := b.addNode k
-  let (b, exid) := b.addNode .exit
-  let b := b.addEdge enid stid
-  let b := b.addEdge stid exid
-  { builder := b, entry := enid, exit := exid }
+-- could the builder carry invariants about the current CFG shape and
+-- edges formation, to avoid rebuilding over and over again?
+structure CFGBuilder where
+  cfg : CFG
+  nextID : NodeID
 
-def seq (r₁ r₂ : BuildResult) : BuildResult :=
-  let ofst := r₁.builder.nextId
-  let n₂ := r₂.builder.cfg.nodes
-  let e₂ := r₂.builder.cfg.edges.map (fun ⟨s, d, k⟩ => ⟨s + ofst, d + ofst, k⟩)
-  let combined := {
-    cfg := {
-      nodes := r₁.builder.cfg.nodes ++ n₂
-      edges := r₁.builder.cfg.edges ++ e₂ ++ [⟨r₁.exit, r₂.entry + ofst, .normal⟩]
-      entry := r₁.entry
-      exit := r₂.exit + ofst
-    }
-    nextId := ofst + r₂.builder.nextId
-  }
-  { builder := combined, entry := r₁.entry, exit := r₂.exit + ofst}
+namespace CFGBuilder
+def empty : CFGBuilder := {
+  cfg := ⟨[], [], 0, 0⟩
+  nextID := 0
+}
 
-def ite (c : Expr) (t f : BuildResult) : BuildResult :=
-  let (b, enid) := CFGBuilder.empty.addNode .entry
-  let (b, cid) := b.addNode (.cond c)
-  let (b, exid) := b.addNode .exit
-  let b := b.addEdge enid cid
-  -- t ofst
-  let tofst := b.nextId
-  let tn := t.builder.cfg.nodes
-  let te := t.builder.cfg.edges.map fun ⟨s, d, l⟩ =>
-    ⟨s + tofst, d + tofst, l⟩
-  let b : CFGBuilder := {
-    cfg := { nodes := b.cfg.nodes ++ tn, edges := b.cfg.edges ++ te,
-             entry := enid, exit := exid }
-    nextId := b.nextId + t.builder.nextId
-  }
-  -- f ofst
-  let fofst := b.nextId
-  let fn := f.builder.cfg.nodes
-  let fe := f.builder.cfg.edges.map fun ⟨s, d, l⟩ =>
-    ⟨s + fofst, d + fofst, l⟩
-  let b : CFGBuilder := {
-    cfg := {
-      nodes := b.cfg.nodes ++ fn
-      edges := b.cfg.edges ++ fe ++
-        [⟨cid, t.entry + tofst, .trueBranch⟩,
-         ⟨cid, f.entry + fofst, .falseBranch⟩,
-         ⟨t.exit + tofst, exid, .normal⟩,
-         ⟨f.exit + fofst, exid, .normal⟩]
-      entry := enid
-      exit := exid
-    }
-    nextId := b.nextId + f.builder.nextId
-  }
-  { builder := b, entry := enid, exit := exid }
+def addNode (b : CFGBuilder) (k : NodeKind) : (CFGBuilder × NodeID) := ({
+  cfg := { b.cfg with nodes := b.cfg.nodes ++ [k] }
+  nextID := b.nextID + 1
+}, b.nextID)
 
-def whil (c : Expr) (body : BuildResult) : BuildResult :=
-  let (b, enid) := CFGBuilder.empty.addNode .entry
-  let (b, cid) := b.addNode (.cond c)
-  let (b, exid) := b.addNode .exit
-  let b := b.addEdge enid cid
-  -- t ofst
-  let bofst := b.nextId
-  let bn := body.builder.cfg.nodes
-  let be := body.builder.cfg.edges.map fun ⟨s, d, l⟩ =>
-    ⟨s + bofst, d + bofst, l⟩
-  let b : CFGBuilder := {
-    cfg := {
-      nodes := b.cfg.nodes ++ bn,
-      edges := b.cfg.edges ++ be ++ [
-        ⟨cid, body.entry + bofst, .trueBranch⟩,
-        ⟨cid, exid, .falseBranch⟩,
-        ⟨body.exit + bofst, cid, .normal⟩
-      ],
-      entry := enid, exit := exid }
-    nextId := b.nextId + body.builder.nextId
-  }
-  { builder := b, entry := enid, exit := exid }
+def addEdge (b : CFGBuilder) (s d : NodeID) (k : EdgeKind) : CFGBuilder := {
+  b with cfg := { b.cfg with edges := b.cfg.edges ++ [⟨s, d, k⟩] }
+}
 
-end BuildResult
-
-def BuildResult.skip : BuildResult :=
-  let (b, enid) := CFGBuilder.empty.addNode .skip
-  let (b, exid) := b.addNode .exit
-  let b := b.addEdge enid exid
-  { builder := b, entry := enid, exit := exid }
-
-def Stmt.buildCFG : Stmt -> BuildResult
-| .Assign x e => BuildResult.single (.assign x e)
-| .Skip => BuildResult.skip
-| .Seq s₁ s₂ => BuildResult.seq s₁.buildCFG s₂.buildCFG
-| .While c b => BuildResult.whil c b.buildCFG
-| .If c t f => BuildResult.ite c t.buildCFG f.buildCFG
-
-def BuildResult.toCFG (b : BuildResult) : CFG :=
-  {b.builder.cfg with entry := b.entry, exit := b.exit}
+def buildGraph (b : CFGBuilder) (s : Stmt) : (CFGBuilder × (Nat × Nat)) :=
+  match s with
+  | .Skip =>
+    let (b, n) := b.addNode .Skip
+    (b, (n, n))
+  | .Decl x e =>
+    let (b, n) := b.addNode (.Decl x e)
+    (b, (n, n))
+  | .Assign x e =>
+    let (b, n) := b.addNode (.Assign x e)
+    (b, (n, n))
+  | .Seq s₁ s₂ =>
+    let (b, (nen₁, nex₁)) := b.buildGraph s₁
+    let (b, (nen₂, nex₂)) := b.buildGraph s₂
+    let b := b.addEdge nex₁ nen₂ .Normal
+    (b, (nen₁, nex₂))
+  | .While cond body =>
+    let (b, nenc) := b.addNode (.Cond cond)
+    let (b, (nenb, nexb)) := b.buildGraph body
+    let (b, nex) := b.addNode .Skip
+    let b := b.addEdge nenc nenb .TBranch
+    let b := b.addEdge nexb nenc .Normal
+    let b := b.addEdge nenc nex .FBranch
+    (b, (nenc, nexb))
+  | .If c t f =>
+    let (b, nenc) := b.addNode (.Cond c)
+    let (b, (nent, next)) := b.buildGraph t
+    let (b, (nenf, nexf)) := b.buildGraph f
+    let (b, nexit) := b.addNode .Skip
+    let b := b.addEdge nenc nent .TBranch
+    let b := b.addEdge nenc nenf .FBranch
+    let b := b.addEdge next nexit .Normal
+    let b := b.addEdge nexf nexit .Normal
+    (b, (nenc, nexit))
+end CFGBuilder
